Azurite/AzInt/Mul.lean
@@ -1,0 +1,21 @@
+import Azurite.AzInt.Add
+import Azurite.AzNat.Mul
+
+namespace Azurite.AzInt
+
+/-- Multiply an `AzInt` `z` by a `UInt64` `u`. -/
+def mulUInt64 (z : AzInt) (u : UInt64) : AzInt :=
+  mkNorm z.sign (z.abs.mulUInt64 u)
+
+/-- Multiply an `AzInt` `z` by an `Int64` `i`. -/
+def mulInt64 (z : AzInt) (i : Int64) : AzInt :=
+  if i ≥ 0 then mkNorm z.sign (z.abs.mulUInt64 i.toUInt64)
+  else mkNorm (!z.sign) (z.abs.mulUInt64 (-i).toUInt64)
+
+/-- Multiply two `AzInt`s. -/
+def mul (a b : AzInt) : AzInt :=
+  mkNorm (a.sign == b.sign) (a.abs * b.abs)
+
+instance : Mul AzInt := ⟨mul⟩
+
+end Azurite.AzInt
