Azurite/AzNat/Instances.lean
@@ -1,0 +1,20 @@
+import Azurite.AzNat.Equiv.Mul
+
+namespace Azurite.AzNat
+
+instance : CommSemiring AzNat where
+  add_assoc a b c := toNat_injective (by simp [toNat_add, Nat.add_assoc])
+  zero_add a := toNat_injective (by simp [toNat_add])
+  add_zero a := toNat_injective (by simp [toNat_add])
+  add_comm a b := toNat_injective (by simp [toNat_add, Nat.add_comm])
+  mul_assoc a b c := toNat_injective (by simp [toNat_mul, Nat.mul_assoc])
+  one_mul a := toNat_injective (by simp [toNat_mul])
+  mul_one a := toNat_injective (by simp [toNat_mul])
+  left_distrib a b c := toNat_injective (by simp [toNat_add, toNat_mul, Nat.mul_add])
+  right_distrib a b c := toNat_injective (by simp [toNat_add, toNat_mul, Nat.add_mul])
+  zero_mul a := toNat_injective (by simp [toNat_mul])
+  mul_zero a := toNat_injective (by simp [toNat_mul])
+  mul_comm a b := toNat_injective (by simp [toNat_mul, Nat.mul_comm])
+  nsmul := nsmulRec
+
+end Azurite.AzNat
